Add support for boxed integers (#22)

theories/examples/gmtime.v
@@ -45,7 +45,7 @@ Section FFI_spec.
 
   Definition caml_gmtime_code (t : expr) : expr :=
     CAMLlocal: "res" in
-    let: "timer" := Int_val (t) in
+    let: "timer" := BoxedInt_val (t) in
     let: "tm"    := (call: &"gmtime" with ("timer")) in
     "res" <- caml_alloc (#2, #0);;
 
@@ -63,7 +63,7 @@ Section FFI_spec.
   Definition caml_gmtime_spec : protocol ML_lang.val Σ :=
     !! (t : Z)
       {{ True }}
-        "caml_gmtime" with [(#ML t)]
+        "caml_gmtime" with [(#ML (ML_lang.LitBoxedInt t))]
       {{
         (tm_sec : Z) (tm_min : Z), RET((#ML tm_sec, #ML tm_min)%MLV);
         True
@@ -80,14 +80,18 @@ Section FFI_spec.
     destruct lvs as [|lv []]; try by (exfalso; eauto with lia); []. clear Hlen.
     destruct ws as [|w []]; try by (exfalso; apply Forall2_length in Hrepr; eauto with lia); [].
     apply Forall2_cons_1 in Hrepr as [Hrepr _].
-    cbn. iDestruct "Hsim" as "[-> _]".
+    cbn.
+    iDestruct "Hsim" as "[Hγ _]".
+    iDestruct "Hγ" as (γ) "[-> Hγ]".
     wp_call_direct.
 
     (* Declare result variable *)
     wp_apply (wp_CAMLlocal with "HGC"); eauto. iIntros (ℓ) "(HGC&Hℓ)". wp_pures.
 
     (* Call stdlib gmtime *)
-    wp_apply (wp_val2int with "HGC"); eauto. iIntros "HGC". wp_pures.
+    wp_apply (wp_read_foreign with "[$HGC $Hγ]"); try eauto.
+    iIntros "(HGC&_)".
+    wp_pures.
     wp_extern. iModIntro. iRight.
     iSplit; first done.
     iExists t; do 2 (iSplit; first done).
@@ -97,7 +101,7 @@ Section FFI_spec.
 
     (* Allocate result variable *)
     wp_apply (wp_alloc (TagDefault) with "HGC"); try done; auto.
-    iIntros (θ' γ' w0') "(HGC&Hγ&%H2)".
+    iIntros (θ' γ' w0') "(HGC&Hγ'&%H2)".
     wp_apply (store_to_root with "[$HGC $Hℓ]"); try done.
     iIntros "(HGC&Hℓ)". wp_pures.
 
@@ -116,16 +120,16 @@ Section FFI_spec.
     (* Load tm_sec *)
     wp_apply (load_from_root with "[$HGC $Hℓ]").
     iIntros (w2) "(Hℓ&HGC&%Hγ2)".
-    wp_apply (wp_modify with "[$HGC $Hγ]"); try eauto.
+    wp_apply (wp_modify with "[$HGC $Hγ']"); try eauto.
     1: simpl; done.
-    iIntros "(HGC&Hγ)". wp_pures.
+    iIntros "(HGC&Hγ')". wp_pures.
 
     (* Load tm_min *)
     wp_apply (load_from_root with "[$HGC $Hℓ]").
     iIntros (w3) "(Hℓ&HGC&%Hγ3)".
-    wp_apply (wp_modify with "[$HGC $Hγ]"); try eauto.
+    wp_apply (wp_modify with "[$HGC $Hγ']"); try eauto.
     1: simpl; done.
-    iIntros "(HGC&Hγ)". wp_pures.
+    iIntros "(HGC&Hγ')". wp_pures.
 
     (* Return *)
     wp_apply (load_from_root with "[$HGC $Hℓ]").
@@ -156,7 +160,7 @@ Section ML_spec.
   Context `{!logrelG Σ}.
 
   Definition program_type_ctx : program_env :=
-    {[ "caml_gmtime" := FunType [ TNat ] (TProd TNat TNat) ]}.
+    {[ "caml_gmtime" := FunType [ TBoxedNat ] (TProd TNat TNat) ]}.
 
   Lemma gmtime_well_typed Δ : ⊢ ⟦ program_type_ctx ⟧ₚ* ⟨∅, caml_gmtime_spec⟩ Δ.
   Proof.
@@ -166,7 +170,8 @@ Section ML_spec.
     iPoseProof (big_sepL2_length with "Hargs") as "%Heq".
     destruct vv as [|v [|??]]; cbn in Heq; try lia.
     cbn. iDestruct "Hargs" as "((%n&->)&_)".
-    iSplit; first done. iExists n.
+    iSplit; first done.
+    iExists n.
     do 2 (iSplit; first done).
     iIntros "!>" (tm_sec tm_min) "_". wp_pures. iModIntro.
     iApply ("HCont" with "[-Htok] Htok").
@@ -174,7 +179,6 @@ Section ML_spec.
     iSplit; first done.
     iSplit; iExists _; done.
   Qed.
-
 
 End ML_spec.
 
@@ -186,7 +190,7 @@ Section ML_Example.
   Context `{!ffiG Σ}.
 
   Definition gmtime_client : mlanguage.expr (lang_to_mlang ML_lang) :=
-    (Fst (Extern "caml_gmtime" [ (Val #0)%MLE ])).
+    (Fst (Extern "caml_gmtime" [ (Val #(LitBoxedInt 0))%MLE ])).
 
   Lemma ML_prog_correct_axiomatic :
     ⊢ WP gmtime_client at ⟨∅, caml_gmtime_spec⟩ {{ v, ⌜∃x : Z, v = #x⌝}}.
