theories/interop/basics.v
@@ -99,21 +99,27 @@ Qed.
 Notation vblock :=
   (ismut * (vblock_tag * list lval))%type.
 
+Notation fblock :=
+  (ismut * option C_intf.val)%type.
+
 (** a block in the block-level store *)
 Inductive block :=
   | Bvblock (vblk : vblock)
   | Bclosure (clos_f clos_x : binder) (clos_body : ML_lang.expr)
   (** A limited form of OCaml's "custom blocks", storing a C value *)
-  | Bforeign (ptr : option C_intf.val).
+  | Bforeign (fblk : fblock).
 
 Definition vblock_mutability (vb: vblock) : ismut :=
   let '(i,_) := vb in i.
+
+Definition fblock_mutability (fb: fblock) : ismut :=
+  let '(i,_) := fb in i.
 
 Definition mutability (b: block) : ismut :=
   match b with
   | Bvblock vblk => vblock_mutability vblk
   | Bclosure _ _ _ => Immut
-  | Bforeign _ => Mut
+  | Bforeign fblk => fblock_mutability fblk
   end.
 
 Definition vblock_get_tag (vb: vblock) : vblock_tag :=
@@ -184,8 +190,10 @@ Definition lloc_map_inj χ :=
    only legal as long as the mutable block has not been "observable" by other
    code than the wrapper..) *)
 Inductive freeze_block : block → block → Prop :=
-  | freeze_block_mut tgvs m' :
-    freeze_block (Bvblock (Mut, tgvs)) (Bvblock (m', tgvs))
+  | freeze_block_mut tgvs :
+    freeze_block (Bvblock (Mut, tgvs)) (Bvblock (Immut, tgvs))
+  | freeze_block_foreign w :
+    freeze_block (Bforeign (Mut, w)) (Bforeign (Immut, w))
   | freeze_block_refl b :
     freeze_block b b.
 
@@ -291,6 +299,9 @@ Inductive is_val : lloc_map → lstore → val → lval → Prop :=
   | is_val_unit χ ζ :
     is_val χ ζ (ML_lang.LitV ML_lang.LitUnit) (Lint 0)
   (** locations *)
+  | is_val_boxedint χ ζ γ x :
+    ζ !! γ = Some (Bforeign (Immut, Some (C_intf.LitV (C_intf.LitInt x)))) →
+    is_val χ ζ (ML_lang.LitV (ML_lang.LitBoxedInt x)) (Lloc γ)
   | is_val_loc χ ζ ℓ γ :
     χ !! γ = Some (LlocPublic ℓ) →
     is_val χ ζ (ML_lang.LitV (ML_lang.LitLoc ℓ)) (Lloc γ)
@@ -547,13 +558,12 @@ Lemma lstore_immut_blocks_lookup_Some ζ γ b :
   lstore_immut_blocks ζ !! γ = Some b ↔ ζ !! γ = Some b ∧ mutability b = Immut.
 Proof.
   rewrite /lstore_immut_blocks map_filter_lookup /=.
-  set X := (ζ !! γ). destruct (ζ !! γ) as [[[i' ?]| |]|] eqn:HH; subst X; cbn;
+  set X := (ζ !! γ). destruct (ζ !! γ) as [[[i' ?]| |[i' ?]]|] eqn:HH; subst X; cbn;
       try naive_solver.
-  { destruct (decide (i' = Immut)); subst.
-    { rewrite option_guard_True //. naive_solver. }
-    { rewrite option_guard_False //. naive_solver. } }
-  { rewrite option_guard_True //. naive_solver. }
-  { rewrite option_guard_False //. naive_solver. }
+  2: rewrite option_guard_True //; naive_solver.
+  all: destruct (decide (i' = Immut)); subst.
+  1, 3: rewrite option_guard_True //; naive_solver.
+  all: rewrite option_guard_False //; naive_solver.
 Qed.
 
 Lemma lstore_immut_blocks_lookup_notin ζ γ :
@@ -702,18 +712,19 @@ Proof.
   apply freeze_block_refl.
 Qed.
 
-Lemma freeze_lstore_freeze_lloc ζ ζ' γ b :
+Lemma freeze_lstore_freeze_lloc ζ ζ' γ b1 b2 :
+  freeze_block b1 b2 →
   freeze_lstore ζ ζ' →
-  ζ' !! γ = Some (Bvblock (Mut, b)) →
-  freeze_lstore ζ (<[γ:=Bvblock (Immut, b)]> ζ').
+  ζ' !! γ = Some b1 →
+  freeze_lstore ζ (<[γ:=b2]> ζ').
 Proof.
-  intros [HL HR] Hζ'γ. split.
+  intros HB [HL HR] Hζ'γ. split.
   - rewrite HL. rewrite dom_insert_L. rewrite subseteq_union_1_L. 1:done.
     intros ? ->%elem_of_singleton. by eapply elem_of_dom.
-  - intros γ1 b1 b2 H1 H2. destruct (decide (γ = γ1)) as [<- |H3].
+  - intros γ1 b1' b2' H1 H2. destruct (decide (γ = γ1)) as [<- |H3].
     * rewrite lookup_insert in H2. injection H2; intros <-.
-      specialize (HR γ b1 (Bvblock (Mut, b)) H1 Hζ'γ).
-      inversion HR; subst; econstructor.
+      specialize (HR γ b1' b1 H1 Hζ'γ).
+      inversion HR; subst; destruct HB; try econstructor; try inversion HR; try econstructor.
     * rewrite lookup_insert_ne in H2; last done. by eapply HR.
 Qed.
 
@@ -788,7 +799,7 @@ Lemma is_val_insert_immut χ ζ γ bb bb2 x y :
 Proof.
   intros H1 H2; induction 1; econstructor; eauto.
   all: rewrite lookup_insert_ne; first done.
-  all: intros ->; destruct bb2 as [[mut [? ?]]| |]; cbn in *.
+  all: intros ->; destruct bb2 as [[mut ?]| |[mut ?]]; cbn in *.
   all: congruence.
 Qed.
 
@@ -968,20 +979,24 @@ Proof.
   eapply expose_llocs_insert; eauto.
 Qed.
 
-Lemma is_store_freeze_lloc χ ζ σ γ b:
+Lemma is_store_freeze_lloc χ ζ σ γ b1 b2:
   is_store χ ζ σ →
+  freeze_block b1 b2 →
   χ !! γ = Some LlocPrivate →
-  ζ !! γ = Some (Bvblock (Mut, b)) →
-  is_store χ (<[γ:=Bvblock (Immut, b)]> ζ) σ.
+  ζ !! γ = Some b1 →
+  is_store χ (<[γ:=b2]> ζ) σ.
 Proof.
-  intros Hstore Hpriv Hζγ l vs' γ1 bb H1 H2 H3.
+  intros Hstore Hfreeze Hpriv Hζγ l vs' γ1 bb H1 H2 H3.
   destruct (decide (γ = γ1)) as [<- | H4].
   * simplify_map_eq.
   * rewrite lookup_insert_ne in H3; last done.
     specialize (Hstore _ _ _ _ H1 H2 H3).
     inversion Hstore. subst vs bb.
     econstructor. eapply Forall2_impl; first done.
-    intros x y H5. eapply is_val_insert_immut; eauto.
+    intros x y H5. destruct Hfreeze.
+    1, 2: eapply is_val_insert_immut; eauto.
+    assert ((<[γ:=b]> ζ) = ζ) as Hζ. { by apply insert_id. }
+    by rewrite Hζ.
 Qed.
 
 Lemma is_store_alloc_block χ σ ζσ ζ γ blk :
@@ -1083,7 +1098,6 @@ Lemma lval_in_vblock v m tg vs :
   lval_in_block (Bvblock (m, (tg, vs))) v ↔ v ∈ vs.
 Proof. split. by inversion 1. intros; by constructor. Qed.
 
-
 Lemma GC_correct_transport ζ1 ζ2 θ : freeze_lstore ζ1 ζ2 → GC_correct ζ1 θ → GC_correct ζ2 θ.
 Proof.
   intros (H1L&H1R) (H2&H3). split; first done.
@@ -1091,9 +1105,10 @@ Proof.
   destruct (ζ1 !! γ) as [b|] eqn:Heq.
   2: { eapply elem_of_dom_2 in HH2. eapply not_elem_of_dom in Heq. rewrite H1L in Heq; tauto. }
   specialize (H1R _ _ _ Heq HH2). inversion H1R; subst.
-  2: { eapply H3; done. }
+  3: { eapply H3; done. }
   destruct tgvs. eapply lval_in_vblock in HH3.
   eapply H3. 1: exact HH1. 1: done. eapply lval_in_vblock. done.
+  inversion HH3.
 Qed.
 
 Lemma GC_correct_transport_rev ζ1 ζ2 θ : freeze_lstore ζ2 ζ1 → GC_correct ζ1 θ → GC_correct ζ2 θ.
@@ -1103,9 +1118,10 @@ Proof.
   destruct (ζ1 !! γ) as [b|] eqn:Heq.
   2: { eapply elem_of_dom_2 in HH2. eapply not_elem_of_dom in Heq. rewrite -H1L in Heq; tauto. }
   specialize (H1R _ _ _ HH2 Heq). inversion H1R; subst.
-  2: { eapply H3; done. }
+  3: { eapply H3; done. }
   destruct tgvs. eapply lval_in_vblock in HH3.
   eapply H3. 1: exact HH1. 1: done. eapply lval_in_vblock. done.
+  inversion HH3.
 Qed.
 
 Lemma GC_correct_modify_block ζ θ γ blk blk' i v w :
@@ -1125,10 +1141,10 @@ Proof using.
   { eapply GC2; eauto. by constructor. }
 Qed.
 
-Lemma GC_correct_modify_foreign ζ θ γ w w' :
-  ζ !! γ = Some (Bforeign w) →
+Lemma GC_correct_modify_foreign ζ θ γ blk blk' :
+  ζ !! γ = Some (Bforeign blk) →
   GC_correct ζ θ →
-  GC_correct (<[γ := Bforeign w']> ζ) θ.
+  GC_correct (<[γ := Bforeign blk']> ζ) θ.
 Proof using.
   intros Hγ [GC1 GC2]. split; first done.
   intros γ0 blk1 γ1 Hγ0 [[??]|[Hne1 Hlu]]%lookup_insert_Some Hlloc; subst; eauto.
