theories/examples/box.v
@@ -70,7 +70,7 @@ Section Proofs.
   Solve Obligations with solve_proper.
 
   Program Definition box_interp : (protocol ML_lang.val Σ) -n> (listO D -n> D) -d> listO D -n> D := λne Ψ, λ interp, λne Δ, PersPred (
-    λ v, ∃ (γ:nat) (ℓ:loc), ⌜v = #(LitForeign γ)⌝ ∗ γ ↦foreign{DfracDiscarded} (#C ℓ) ∗
+    λ v, ∃ (γ:nat) (ℓ:loc), ⌜v = #(LitForeign γ)⌝ ∗ γ ↦foreign[Immut] (#C ℓ) ∗
            na_inv logrel_nais (nroot .@ "value"   .@ γ) (box_invariant_1 (ℓ +ₗ 1) (interp Δ)) ∗
            na_inv logrel_nais (nroot .@ "callback".@ γ) (box_invariant_2 ℓ (interp_arrow ⟨ ∅ , Ψ ⟩ interp interp_unit Δ)))%I.
   Next Obligation. solve_proper. Qed.
@@ -119,7 +119,7 @@ Section Proofs.
     iIntros (s ws Φ) "H". iNamed "H". iNamedProto "Hproto".
     iSplit; first done.
     destruct lvs as [|lvl [|??]]; try done.
-    all: cbn; iDestruct "Hsim" as "(Hsimv&Hsim)"; try done.
+    all: iEval (cbn) in "Hsim"; iDestruct "Hsim" as "(Hsimv&Hsim)"; try done.
     destruct ws as [|wv [|??]]; decompose_Forall.
     iIntros (Φ'') "Cont2".
     wp_pure _.
@@ -139,17 +139,17 @@ Section Proofs.
     wp_pures.
     wp_apply (wp_write_foreign with "[$HGC $Hγfgn]"); [done..|].
     iIntros "(HGC&Hγfgn)". wp_pures.
-    iDestruct "Hγfgn" as "(Hγfgn'&_)".
+    iDestruct "Hγfgn" as "(Hγfgn'&Hγfresh)".
     iMod (na_inv_alloc logrel_nais _ _ (box_invariant_1 (ℓ +ₗ 1) (interp Δ)) with "[Hℓ1]") as "#Hinv1".
     { iNext. iExists _, _. iFrame "Hℓ1 Hsimv Hv". }
     iMod (na_inv_alloc logrel_nais _ _ (box_invariant_2 ℓ (interp_arrow ⟨ ∅ , Ψ ⟩ interp interp_unit Δ)) with "[Hℓ0]") as "#Hinv2".
     { iNext. iRight. iFrame. }
-    iMod (ghost_map.ghost_map_elem_persist with "Hγfgn'") as "#Hγfgn'".
+    iMod (freeze_foreign_to_immut γ θ1 _ with "[$]") as "(HGC&#Hγfgn)".
     iModIntro. iApply "Cont2". iApply ("Return" $! θ1 (#(LitForeign γ)) with "HGC [-] [] []").
     2,3: done.
     iApply "Cont". iFrame "Hna". iExists γ, ℓ.
-    iSplit; first done. iSplitL.
-    { iSplitL. 2: done. iApply "Hγfgn'". }
+    iSplit; first done. 
+    iSplitL; first done.
     iFrame "Hinv1 Hinv2".
   Qed.
 
@@ -159,8 +159,8 @@ Section Proofs.
     iIntros (s ws Φ) "H". iNamed "H". iNamedProto "Hproto".
     iSplit; first done.
     destruct lvs as [|lvn [|lvb [|??]]]; try done.
-    all: cbn; iDestruct "Hsim" as "(Hsimvn&Hsim)"; try done.
-    all: cbn; iDestruct "Hsim" as "(Hsimvb&Hsim)"; try done.
+    all: iEval (cbn) in "Hsim"; iDestruct "Hsim" as "(Hsimvn&Hsim)"; try done.
+    all: iEval (cbn) in "Hsim"; iDestruct "Hsim" as "(Hsimvb&Hsim)"; try done.
     destruct ws as [|wn [|wb [|??]]]; decompose_Forall.
     iIntros (Φ'') "Cont2".
     wp_pure _.
@@ -209,15 +209,14 @@ Section Proofs.
       iApply ("Return" with "HGC (Cont Hna) [//] [//]").
   Qed.
 
-
   Lemma box_listen_correct :
     prims_proto Ψ ||- box_prog :: wrap_proto box_listen_spec_ML.
   Proof.
     iIntros (s ws Φ) "H". iNamed "H". iNamedProto "Hproto".
     iSplit; first done.
     destruct lvs as [|lv [|lvb [|??]]]; try done.
-    all: cbn; iDestruct "Hsim" as "(Hsimvl&Hsim)"; try done.
-    all: cbn; iDestruct "Hsim" as "(Hsimvb&Hsim)"; try done.
+    all: iEval (cbn) in "Hsim"; iDestruct "Hsim" as "(Hsimvl&Hsim)"; try done.
+    all: iEval (cbn) in "Hsim"; iDestruct "Hsim" as "(Hsimvb&Hsim)"; try done.
     destruct ws as [|wl [|wb [|??]]]; decompose_Forall.
     iIntros (Φ'') "Cont2".
     wp_pure _.
@@ -253,6 +252,7 @@ Section Proofs.
       iIntros (w0) "(HGC&%Hw0)". iApply "Cont2".
       iApply ("Return" with "HGC (Cont Hna) [//] [//]").
   Qed.
+
   End InPsi.
 
   Definition box_prog_spec_ML (Ψ : protocol ML_lang.val Σ) : protocol ML_lang.val Σ :=
@@ -280,6 +280,7 @@ Section Proofs.
   Proof.
     exact (fixpoint_unfold (box_prog_spec_ML) s vv Φ).
   Qed.
+
   Lemma buf_library_spec_ML_sim:
    (box_prog_spec_ML (box_spec_ML) ⊑ box_spec_ML)%I.
   Proof.
