theories/examples/listener.v
@@ -72,7 +72,7 @@ Section Proofs.
   Solve Obligations with solve_proper.
 
   Program Definition listener_interp : (protocol ML_lang.val Σ) -n> (listO D -n> D) -d> listO D -n> D := λne Ψ, λ interp, λne Δ, PersPred (
-    λ v, ∃ γ (a:addr), ⌜v = #(LitForeign γ)⌝ ∗ γ ↦foreign{DfracDiscarded} (#C a) ∗
+    λ v, ∃ γ (a:addr), ⌜v = #(LitForeign γ)⌝ ∗ γ ↦foreign[Immut] (#C a) ∗
            na_inv logrel_nais (nroot .@ "listener" .@ γ)
              (listener_invariant a (interp_arrow ⟨ ∅ , Ψ ⟩ interp interp_unit Δ)))%I.
   Next Obligation. solve_proper. Qed.
@@ -129,7 +129,7 @@ Section Proofs.
     iIntros (s ws Φ) "H". iNamed "H". iNamedProto "Hproto".
     iSplit; first done.
     destruct lvs as [|lvl [|??]]; try done.
-    all: cbn; iDestruct "Hsim" as "(->&Hsim)"; try done.
+    all: iEval (cbn) in "Hsim"; iDestruct "Hsim" as "(->&Hsim)"; try done.
     destruct ws as [|wv [|??]]; decompose_Forall.
     iIntros (Φ'') "Cont2".
     wp_pure _.
@@ -145,15 +145,15 @@ Section Proofs.
     wp_pures.
     wp_apply (wp_write_foreign with "[$HGC $Hγfgn]"); [done..|].
     iIntros "(HGC&Hγfgn)". wp_pures.
-    iDestruct "Hγfgn" as "(Hγfgn'&_)".
+    iDestruct "Hγfgn" as "(Hγfgn'&Hγfresh)".
     iMod (na_inv_alloc logrel_nais _ _ (listener_invariant a _) with "[Ha]") as "#Hinv".
     { iNext. iRight. iFrame "Ha". }
-    iMod (ghost_map.ghost_map_elem_persist with "Hγfgn'") as "#Hγfgn'".
+    iMod (freeze_foreign_to_immut γ θ1 _ with "[$]") as "(HGC&#Hγfgn')".
     iModIntro. iApply "Cont2". iApply ("Return" $! θ1 (#(LitForeign γ)) with "HGC [-] [] []").
     2,3: done.
     iApply "Cont". iFrame "Hna". iExists γ, a.
     iSplit; first done. iSplitL.
-    { iSplitL. 2: done. iApply "Hγfgn'". }
+    { iApply "Hγfgn'". }
     iFrame "Hinv".
   Qed.
 
@@ -195,7 +195,7 @@ Section Proofs.
       iApply "Cont2". iApply ("Return" with "HGC [Cont Hna] [] []").
       1: by iApply "Cont". 1,2: by iPureIntro.
     - wp_apply (wp_load with "[$Hnull]"). iIntros "Hnull".
-      wp_pures. 
+      wp_pures.
       iMod ("Hclose" with "[$Hna Hnull]") as "Hna".
       { iNext. iRight. iFrame. }
       wp_apply (wp_int2val with "HGC"); [done..|].
@@ -260,7 +260,7 @@ Section Proofs.
     iIntros (s ws Φ) "H". iNamed "H". iNamedProto "Hproto".
     iSplit; first done.
     destruct lvs as [|lv [|lvb [|??]]]; try done.
-    all: cbn; iDestruct "Hsim" as "(Hsimvb&Hsim)"; try done.
+    all: iEval (cbn) in "Hsim"; iDestruct "Hsim" as "(Hsimvb&Hsim)"; try done.
     destruct ws as [|wl [|wb [|??]]]; decompose_Forall.
     iIntros (Φ'') "Cont2".
     wp_pure _.
@@ -298,6 +298,7 @@ Section Proofs.
       iApply "Cont2". iApply ("Return" with "HGC [Cont Hna]").
       1: by iApply "Cont". 1,2: by iPureIntro.
   Qed.
+
   End InPsi.
 
   Definition listener_prog_spec_ML (Ψ : protocol ML_lang.val Σ) : protocol ML_lang.val Σ :=
@@ -350,7 +351,7 @@ Section Proofs.
                                                          (λ: "v1" "v2", extern: "listener_listen" with ("v1", "v2")),
                                                          (λ: "v1", extern: "listener_unlisten" with ("v1"))).
 
-  
+
   Definition ML_type_inner (t:type) : type :=
     (TProd (TProd (TProd
        (* unit -> 'a listener *)
@@ -422,7 +423,7 @@ Section Proofs.
     let: <> := Snd (Fst "l") (λ: "v", Snd (Fst (Fst "l")) (#1) "ml") "ml" in
     #42.
 
-  Lemma listener_client_1_typed : 
+  Lemma listener_client_1_typed :
     typed ∅ ∅ listener_client_1 (TArrow ML_type TNat).
   Proof.
     econstructor; cbn in *.
@@ -446,7 +447,7 @@ Section Proofs.
 End Proofs.
 
 
-Lemma listener_client_1_adequacy : 
+Lemma listener_client_1_adequacy :
 umrel.trace (mlanguage.prim_step (combined_prog listener_client listener_prog))
   (LkCall "main" [], adequacy.σ_init)
   (λ '(e, σ), ∃ x, mlanguage.to_val e = Some (code_int x) ∧ True).
