theories/examples/new_boxedint.v
@@ -1,0 +1,122 @@
+From iris.proofmode Require Import coq_tactics reduction spec_patterns.
+From iris.proofmode Require Export tactics.
+From iris.prelude Require Import options.
+From melocoton Require Import named_props.
+From melocoton.ml_lang.logrel Require logrel typing fundamental.
+From melocoton.interop Require Import basics basics_resources.
+From melocoton.lang_to_mlang Require Import lang weakestpre.
+From melocoton.interop Require Import lang weakestpre update_laws wp_utils wp_ext_call_laws wp_simulation.
+From melocoton.c_interop Require Import rules.
+From melocoton.ml_lang Require Import notation lang_instantiation.
+From melocoton.c_lang Require Import mlang_instantiation lang_instantiation.
+From melocoton.ml_lang Require proofmode.
+From melocoton.c_lang Require notation proofmode.
+From melocoton.mlanguage Require Import progenv.
+From melocoton.mlanguage Require weakestpre.
+From melocoton.linking Require Import lang weakestpre.
+From melocoton.combined Require Import adequacy rules.
+
+Section FFI_spec.
+
+  Import melocoton.c_interop.notation melocoton.c_lang.proofmode.
+
+  Context `{SI:indexT}.
+  Context `{!ffiG Σ}.
+
+  Definition caml_new_boxedint_code (t : expr) : expr :=
+    let: "res" := caml_alloc_custom ( ) in
+    (Custom_contents ( "res" ) := #(LitInt 0));;
+    "res".
+
+  Definition caml_new_boxedint_prog : lang_prog C_lang :=
+    {[ "caml_new_boxedint" := Fun [] (caml_new_boxedint_code "t") ]}.
+
+  Definition caml_new_boxedint_spec : protocol ML_lang.val Σ :=
+    !!
+      {{ True }}
+        "caml_new_boxedint" with []
+      {{
+        RET((#ML (LitBoxedInt 0))%MLV);
+        True
+      }}.
+
+  Lemma new_boxedint_correct :
+    prims_proto caml_new_boxedint_spec
+    ||- caml_new_boxedint_prog :: wrap_proto caml_new_boxedint_spec.
+  Proof.
+    iIntros (fn ws Φ) "H". iNamed "H". iNamedProto "Hproto".
+    iSplit; first done. iIntros (Φ'') "HΦ".
+    iAssert (⌜length lvs = 0⌝)%I as %Hlen.
+    { by iDestruct (big_sepL2_length with "Hsim") as %?. }
+    destruct lvs as [|lv []]; try by (exfalso; eauto with lia); []. clear Hlen.
+    destruct ws as [|w []]; try by (exfalso; apply Forall2_length in Hrepr; eauto with lia); [].
+    cbn.
+    wp_call_direct.
+
+    (* Allocate result variable *)
+    wp_apply (wp_alloc_foreign with "[$HGC]"); try eauto.
+    iIntros (θ' γ w) "(HGC&Hγ&%Hγw)". wp_pures.
+
+    (* Populate result variable *)
+    wp_apply (wp_write_foreign with "[$HGC $Hγ]"); try eauto.
+    iIntros "(HGC&Hγ)". wp_pures.
+
+    iMod (freeze_foreign_to_immut γ θ' _ with "[$]") as "(HGC&#Hγ)".
+
+    iModIntro.
+    iApply "HΦ".
+    iApply ("Return" with "[$HGC] [Cont] []").
+    - by iApply "Cont".
+    - cbn. iExists γ. iSplit; try eauto.
+    - eauto.
+Qed.
+
+End FFI_spec.
+
+Section ML_spec.
+  Import melocoton.ml_lang.proofmode.
+  Import logrel typing fundamental.
+
+  Context `{SI:indexT}.
+  Context `{!ffiG Σ}.
+  Context `{!logrelG Σ}.
+
+  Definition program_type_ctx : program_env :=
+    {[ "caml_new_boxedint" := FunType [] (TBoxedNat) ]}.
+
+  Lemma new_boxedint_well_typed Δ : ⊢ ⟦ program_type_ctx ⟧ₚ* ⟨∅, caml_new_boxedint_spec⟩ Δ.
+  Proof.
+    iIntros (s vv Φ) "!> (%ats&%rt&%Heq&Hargs&Htok&HCont)".
+    wp_extern. iModIntro. unfold program_type_ctx in Heq.
+    apply lookup_singleton_Some in Heq as (<-&Heq). simplify_eq.
+    iPoseProof (big_sepL2_length with "Hargs") as "%Heq".
+    destruct vv as [|v [|??]]; cbn in Heq; try lia.
+    cbn.
+    do 3 (iSplit; first done).
+    iIntros "!> _". wp_pures. iModIntro.
+    iApply ("HCont" with "[-Htok] Htok").
+    iExists 0. done.
+  Qed.
+
+End ML_spec.
+
+Section ML_Example.
+
+  Import melocoton.ml_lang.proofmode.
+
+  Context `{SI:indexT}.
+  Context `{!ffiG Σ}.
+
+  Definition new_boxedint_client : mlanguage.expr (lang_to_mlang ML_lang) :=
+    (Extern "caml_new_boxedint" []).
+
+  Lemma ML_prog_correct_axiomatic :
+    ⊢ WP new_boxedint_client at ⟨∅, caml_new_boxedint_spec⟩ {{ v, ⌜∃x : Z, v = #ML (LitBoxedInt x)⌝}}.
+  Proof.
+    unfold new_boxedint_client. wp_pures. wp_extern.
+    iModIntro. cbn.
+    do 3 (iSplitR; first done). iIntros "!> _".
+    wp_pures. iModIntro. iPureIntro. eauto.
+  Qed.
+
+End ML_Example.
