theories/interop/update_laws.v
@@ -55,7 +55,21 @@ Lemma freeze_to_immut γ lvs θ :
 Proof using.
   iIntros "(HGC & Hγ)". iNamed "HGC".
   iDestruct (lstore_own_vblock_F_as_mut with "Hγ") as "([Hmtζ _] & Hmtfresh)".
-  iMod (hgh_freeze_block with "GCHGH Hmtζ Hmtfresh") as "(GCHGH & Hmtζ & Hmtfresh)".
+  assert (freeze_block (Bvblock (Mut, lvs)) (Bvblock (Immut, lvs))) as Hfreeze.
+    { econstructor. }
+  iMod (hgh_freeze_block _ _ _ _ _ _ Hfreeze with "GCHGH Hmtζ Hmtfresh") as "(GCHGH & Hmtζ & Hmtfresh)".
+  iModIntro. iSplitR "Hmtζ Hmtfresh"; last by iFrame; eauto.
+  rewrite /GC /named. repeat iExists _. iFrame; eauto.
+Qed.
+
+Lemma freeze_foreign_to_immut γ θ b :
+  ⊢ GC θ ∗ γ ↦foreign[Mut] b ==∗
+    GC θ ∗ γ ↦foreign[Immut] b.
+Proof.
+  iIntros "(HGC & [Hγ1 Hγ2])". iNamed "HGC".
+  assert (freeze_block (Bforeign (Mut, Some b)) (Bforeign (Immut, Some b))) as Hfreeze.
+    { econstructor. }
+  iMod (hgh_freeze_block _ _ _ _ _ _ Hfreeze with "GCHGH Hγ1 Hγ2") as "(GCHGH & Hmtζ & Hmtfresh)".
   iModIntro. iSplitR "Hmtζ Hmtfresh"; last by iFrame; eauto.
   rewrite /GC /named. repeat iExists _. iFrame; eauto.
 Qed.
